Renaming exported functions (and adding one)

formalization/mfotl/code/Monitor_Code.thy
@@ -984,13 +984,16 @@ instance event_data :: equal by standard
 definition check_all :: "(MFOTL.name \<times> 'd ::  {default,linorder} list) trace \<Rightarrow> 'd MFOTL.formula \<Rightarrow> ('d, 'd proof) pdt \<Rightarrow> bool" where
   "check_all \<sigma> \<phi> e = (distinct_paths e \<and> check_all_aux \<sigma> (\<lambda>_. UNIV) \<phi> e)"
 
-definition check_all_ed :: "(MFOTL.name \<times> event_data list) trace \<Rightarrow> event_data MFOTL.formula \<Rightarrow> (event_data, event_data proof) pdt \<Rightarrow> bool" where
-  "check_all_ed \<sigma> \<phi> e = check_all \<sigma> \<phi> e"
+definition check_all_specialized :: "(MFOTL.name \<times> event_data list) trace \<Rightarrow> event_data MFOTL.formula \<Rightarrow> (event_data, event_data proof) pdt \<Rightarrow> bool" where
+  "check_all_specialized \<sigma> \<phi> e = check_all \<sigma> \<phi> e"
 
-definition trace_of_list_ed :: "((MFOTL.name \<times> event_data list) set \<times> nat) list \<Rightarrow> (MFOTL.name \<times> event_data list) trace" where
-  "trace_of_list_ed xs = trace_of_list xs"
+definition trace_of_list_specialized :: "((MFOTL.name \<times> event_data list) set \<times> nat) list \<Rightarrow> (MFOTL.name \<times> event_data list) trace" where
+  "trace_of_list_specialized xs = trace_of_list xs"
 
-definition ed_set :: "(MFOTL.name \<times> event_data list) list \<Rightarrow> (MFOTL.name \<times> event_data list) set" where
+definition specialized_set :: "(MFOTL.name \<times> event_data list) list \<Rightarrow> (MFOTL.name \<times> event_data list) set" where
+  "specialized_set = set"
+
+definition ed_set :: "event_data list \<Rightarrow> event_data set" where
   "ed_set = set"
 
 lift_definition abs_part :: "(event_data set \<times> 'a) list \<Rightarrow> (event_data, 'a) part" is
@@ -1007,8 +1010,9 @@ lemma check_all_check_one: "check_all \<sigma> \<phi> e = (distinct_paths e \<an
   by (rule conj_cong[OF refl], subst check_all_aux_check_one)
     (auto simp: compatible_vals_def)
 
-export_code check_all_ed trace_of_list_ed interval enat nat_of_integer integer_of_nat
-  STT MFOTL.TT Inl EInt MFOTL.Var Leaf ed_set abs_part
+export_code interval enat nat_of_integer integer_of_nat
+  STT MFOTL.TT Inl EInt MFOTL.Var Leaf 
+  check_all_specialized trace_of_list_specialized specialized_set ed_set abs_part
   in OCaml module_name MFOTL_Explanator2 file_prefix "MFOTL_checker"
 
 end
